theories/DiophantineConstraints/H10UPC.v
@@ -25,22 +25,3 @@ Definition h10upc_sem φ (c : h10upc) :=
 *)
 Definition H10UPC_SAT (cs: list h10upc) := 
   exists (φ: nat -> nat), forall c, In c cs -> h10upc_sem φ c.
-
-Require Import ssreflect Lia.
-
-Lemma h10upc_sem_spec0 {x z1 z2} : 
-  h10upc_sem id ((x, 0), (z1, z2)) <-> 
-  (1 + x = z1 /\ 0 = z2).
-Proof. rewrite /id /=. by lia. Qed.
-
-Lemma h10upc_sem_specS {x y z1 z2} : 
-  h10upc_sem id ((x, S y), (z1, z2)) <-> 
-  (exists z1' n, 
-    h10upc_sem id ((z1', 0), (z1, 0)) /\
-    h10upc_sem id ((x, y), (z1', n)) /\ 
-    h10upc_sem id ((n, y), (z2, n))).
-Proof.
-  constructor.
-  - rewrite /id /= => ?. exists (z1 - 1), (z2 - S y). by nia.
-  - rewrite /id /= => - [?] [?]. by nia.  
-Qed.
